LambdaBox algebra done

LambdaBox.v
@@ -1,14 +1,50 @@
 Require Import Coq.Vectors.Fin.
 Require Import Coq.Vectors.Vector.
 Require Import Coq.Arith.PeanoNat.
+Require Import Coq.Classes.RelationClasses.
+Require Import Coq.Logic.Eqdep_dec.
+Import EqNotations.
 
 Require Import SigmaAlgebra.
 Require Import VarianceLabeledTree.
+Require Import SortEmbeddings.
+Require Import VectorQuantification.
+Require Import Cantor.
 
 Inductive Ty: Set :=
 | Const : nat -> Ty
 | Arrow : Ty -> Ty -> Ty
 | BoxTy : Ty -> Ty.
+
+
+Definition pushVar {m: nat} (Context: Fin.t m -> Ty) (ty: Ty): Fin.t (S m) -> Ty :=
+  fun (x: Fin.t (S m)) =>
+    match x in Fin.t (S k) return (Fin.t k -> Ty) -> Ty with
+    | Fin.F1 => fun _ => ty
+    | Fin.FS k => fun ctxt => ctxt k
+    end Context.
+
+Definition popVar {m: nat} (Context: Fin.t (S m) -> Ty): Fin.t m -> Ty :=
+  fun x => Context (Fin.FS x).
+
+Definition topVarTy {m: nat} (Context: Fin.t (S m) -> Ty): Ty :=
+  Context (Fin.F1).
+
+Lemma pushTopTy_eq:
+  forall {m : nat} (Context: Fin.t m -> Ty) (ty: Ty), topVarTy (pushVar Context ty) = ty.
+Proof.
+  intros m Context ty.
+  reflexivity.
+Qed.
+
+Lemma pushPop_eq:
+  forall {m : nat} (Context: Fin.t m -> Ty) (ty: Ty), popVar (pushVar Context ty) = Context.
+Proof.
+  intros m Context ty.
+  unfold pushVar.
+  unfold popVar.
+  reflexivity.
+Qed.
 
 Inductive LambdaBox: forall {n m} (Delta: Fin.t n -> Ty) (Gamma: Fin.t m -> Ty), Ty -> Type :=
 | Var : forall {n m : nat} (Delta: Fin.t n -> Ty) (Gamma: Fin.t m -> Ty) x, LambdaBox Delta Gamma (Gamma x)
@@ -19,33 +55,203 @@ Inductive LambdaBox: forall {n m} (Delta: Fin.t n -> Ty) (Gamma: Fin.t m -> Ty),
     LambdaBox Delta Gamma tau
 | Lam : forall {n m: nat} (Delta: Fin.t n -> Ty) (Gamma: Fin.t (S m) -> Ty) tau,
     LambdaBox Delta Gamma tau ->
-    LambdaBox Delta (fun x => Gamma (FS x)) (Arrow (Gamma F1) tau)
+    LambdaBox Delta (popVar Gamma) (Arrow (topVarTy Gamma) tau)
 | MLam : forall {n m: nat} (Delta: Fin.t (S n) -> Ty) (Gamma: Fin.t m -> Ty) tau,
     LambdaBox Delta Gamma tau ->
-    LambdaBox (fun x => Delta (FS x)) Gamma (Arrow (Delta F1) tau)
-| Box: forall {n: nat} (Delta: Fin.t n -> Ty) (Gamma: Fin.t 0 -> Ty) tau,
+    LambdaBox (popVar Delta) Gamma (Arrow (topVarTy Delta) tau)
+| Box: forall {n m: nat} (Delta: Fin.t n -> Ty) (Gamma: Fin.t 0 -> Ty) (Gamma': Fin.t m -> Ty) tau,
     LambdaBox Delta Gamma tau ->
-    LambdaBox Delta Gamma (BoxTy tau)
+    LambdaBox Delta Gamma' (BoxTy tau)
 | LetBox: forall {n m: nat} (Delta: Fin.t (S n) -> Ty) (Gamma: Fin.t m -> Ty) sigma,
-    LambdaBox (fun x => Delta (FS x)) Gamma (BoxTy (Delta F1)) ->
+    LambdaBox (popVar Delta) Gamma (BoxTy (topVarTy Delta)) ->
     LambdaBox Delta Gamma sigma ->
-    LambdaBox (fun x => Delta (FS x)) Gamma sigma.
+    LambdaBox (popVar Delta) Gamma sigma.
+
+Definition permute_gamma:
+  forall {m n: nat} (Delta: Fin.t m -> Ty) (Gamma Gamma': Fin.t n -> Ty) sigma,
+    (forall k, { k': _ | Gamma k = Gamma' k' }) ->
+    LambdaBox Delta Gamma sigma ->
+    LambdaBox Delta Gamma' sigma.
+Proof.
+  intros m n Delta Gamma Gamma' sigma gamma_gamma' Msigma.
+  induction Msigma as [ ? ? ? ? x | | | ? ? ? ? ? ? IH | | | ].
+  - destruct (gamma_gamma' x) as [ x' gamma_eq ].
+    rewrite gamma_eq.
+    exact (Var _ _ x').
+  - eapply MVar.
+  - eapply App; eauto.
+  - assert (push_permute: forall k, { k' : Fin.t (S m) | Gamma k = pushVar Gamma' (topVarTy Gamma) k' }).
+    { intro k.
+      apply (Fin.caseS' k).
+      - exists Fin.F1. reflexivity.
+      - intro k'.
+        destruct (gamma_gamma' k') as [ k'' gamma_eq ].
+        exists (Fin.FS k'').
+        simpl.
+        rewrite <- gamma_eq.
+        reflexivity. }     
+    exact (Lam _ _ _ (IH _ push_permute)).
+  - eapply MLam; eauto.
+  - eapply Box; eauto.
+  - eapply LetBox; eauto.
+Defined.
+
+Definition permute_delta:
+  forall {m n: nat} (Delta Delta': Fin.t m -> Ty) (Gamma: Fin.t n -> Ty) sigma,
+    (forall k, { k': _ | Delta k = Delta' k' }) ->
+    LambdaBox Delta Gamma sigma ->
+    LambdaBox Delta' Gamma sigma.
+Proof.
+  intros m n Delta Delta' Gamma sigma delta_delta' Msigma.
+  induction Msigma as [ | ? ? ? ? u | | | ? ? ? ? ? ? IH | | ? ? ? ? ? ? IH ? IH' ].
+  - eapply Var.
+  - destruct (delta_delta' u) as [ u' delta_eq ].
+    rewrite delta_eq.
+    exact (MVar _ _ u').
+  - eapply App; eauto.
+  - eapply Lam; eauto.
+  - assert (push_permute: forall k, { k' : Fin.t (S n) | Delta k = pushVar Delta' (topVarTy Delta) k' }).
+    { intro k.
+      apply (Fin.caseS' k).
+      - exists Fin.F1. reflexivity.
+      - intro k'.
+        destruct (delta_delta' k') as [ k'' delta_eq ].
+        exists (Fin.FS k'').
+        simpl.
+        rewrite <- delta_eq.
+        reflexivity. }     
+    exact (MLam _ _ _ (IH _ push_permute)).
+  - eapply Box; eauto.
+  - assert (push_permute: forall k, { k' : Fin.t (S n) | Delta k = pushVar Delta' (topVarTy Delta) k' }).
+    { intro k.
+      apply (Fin.caseS' k).
+      - exists Fin.F1. reflexivity.
+      - intro k'.
+        destruct (delta_delta' k') as [ k'' delta_eq ].
+        exists (Fin.FS k'').
+        simpl.
+        rewrite <- delta_eq.
+        reflexivity. }
+    exact (LetBox _ _ _ (IH _ delta_delta') (IH' _ push_permute)).
+Defined.
+ 
+
+Definition weaken_gamma:
+  forall {m n: nat} (Delta: Fin.t m -> Ty) (Gamma: Fin.t n -> Ty) sigma tau,
+    LambdaBox Delta Gamma sigma -> LambdaBox Delta (pushVar Gamma tau) sigma.
+Proof.
+  intros m n Delta Gamma sigma tau Msigma.
+  induction Msigma as [ ? ? ? ? x | ? ? ? ? u | | ? ? ? ? sigma ? IH  | | | ].
+  - exact (Var _ _ (Fin.FS x)).
+  - exact (MVar _ _ u).
+  - eapply App; eauto.
+  - assert (IH': LambdaBox Delta (pushVar (pushVar (popVar Gamma) tau) (topVarTy Gamma)) sigma).
+    { eapply permute_gamma; [ | exact IH ].
+      intro k.
+      apply (Fin.caseS' k); clear k.
+      - exists (Fin.FS Fin.F1); reflexivity.
+      - intro k.
+        apply (Fin.caseS' k); clear k.
+        + exists (Fin.F1); reflexivity.
+        + intro k.
+          exists (Fin.FS (Fin.FS k)); reflexivity. }
+    generalize (Lam _ _ _ IH').
+    rewrite pushPop_eq.
+    rewrite pushTopTy_eq.
+    intro; assumption.
+  - eapply MLam; eauto.
+  - eapply Box; eauto.
+  - eapply LetBox; eauto.
+Defined.
+
+Definition weaken_delta:
+  forall {m n: nat} (Delta: Fin.t m -> Ty) (Gamma: Fin.t n -> Ty) sigma tau,
+    LambdaBox Delta Gamma sigma -> LambdaBox (pushVar Delta tau) Gamma sigma.
+Proof.
+  intros m n Delta Gamma sigma tau Msigma.
+  induction Msigma as [ ? ? ? ? x | ? ? ? ? u | | | ? ? ? ? sigma ? IH  | | ? ? ? ? ? ? IH ? IH' ].
+  - exact (Var _ _ x).
+  - exact (MVar _ _ (Fin.FS u)).
+  - eapply App; eauto.
+  - eapply Lam; eauto.
+  - assert (IH': LambdaBox (pushVar (pushVar (popVar Delta) tau) (topVarTy Delta)) Gamma sigma).
+    { eapply permute_delta; [ | exact IH ].
+      intro k.
+      apply (Fin.caseS' k); clear k.
+      - exists (Fin.FS Fin.F1); reflexivity.
+      - intro k.
+        apply (Fin.caseS' k); clear k.
+        + exists (Fin.F1); reflexivity.
+        + intro k.
+          exists (Fin.FS (Fin.FS k)); reflexivity. }
+    generalize (MLam _ _ _ IH').
+    rewrite pushPop_eq.
+    rewrite pushTopTy_eq.
+    intro; assumption.
+  - eapply Box; eauto.
+  - assert (IH_perm: LambdaBox (popVar (pushVar (pushVar (popVar Delta) tau) (topVarTy Delta))) Gamma
+                           (BoxTy (topVarTy Delta))).
+    { eapply permute_delta; [ | exact IH ].
+      intro k.
+      rewrite pushPop_eq.
+      exists k; reflexivity. }
+    assert (topTy_eq: topVarTy Delta = topVarTy (pushVar (pushVar (popVar Delta) tau) (topVarTy Delta))).
+    { rewrite pushTopTy_eq.
+      reflexivity. }
+    rewrite topTy_eq in IH_perm.
+    assert (IH'_perm: LambdaBox (pushVar (pushVar (popVar Delta) tau) (topVarTy Delta)) Gamma sigma).
+    { eapply permute_delta; [ | exact IH' ].
+      intro k.
+      apply (Fin.caseS' k); clear k.
+      - exists (Fin.FS Fin.F1); reflexivity.
+      - intro k.
+        apply (Fin.caseS' k); clear k.
+        + exists (Fin.F1); reflexivity.
+        + intro k.
+          exists (Fin.FS (Fin.FS k)); reflexivity. }
+    generalize (LetBox _ _ _ IH_perm IH'_perm).
+    rewrite pushPop_eq.
+    intro; assumption.
+Defined.
+
+Definition MApp
+           {m n: nat} (Delta: Fin.t m -> Ty) (Gamma: Fin.t n -> Ty)
+           sigma tau
+           (M: LambdaBox Delta Gamma (BoxTy (Arrow sigma tau)))
+           (N: LambdaBox Delta Gamma (BoxTy sigma)): LambdaBox Delta Gamma (BoxTy tau).
+Proof.
+  rewrite <- (pushPop_eq Delta (Arrow sigma tau)).
+  apply LetBox.
+  - rewrite pushPop_eq.
+    rewrite pushTopTy_eq.
+    exact M.
+  - rewrite <- (pushPop_eq _ sigma).
+    apply LetBox.
+    + rewrite pushPop_eq.
+      rewrite pushTopTy_eq.
+      apply weaken_delta.
+      exact N.
+    + apply (Box _ (fun k => Const 0) Gamma).
+      apply (App _ _ sigma).
+      * exact (MVar _ _ (Fin.FS (Fin.F1))).
+      * exact (MVar _ _ Fin.F1).
+Defined.
+
 
 Section ClosedImplementations.
-  Variable EmptyContext : Fin.t 0 -> Ty.
+  Context { EmptyContext : Fin.t 0 -> Ty }.
   Definition Implementations := list { ty : _ & LambdaBox EmptyContext EmptyContext (BoxTy ty) }.
 
   Inductive TyConstr: Set :=
   | TyConstr_Const : nat -> TyConstr
   | TyConstr_Arrow : TyConstr
-  | TyConstr_Box : TyConstr
-  | TyConstr_BlackBox : TyConstr.
+  | TyConstr_Box : TyConstr.
 
   Lemma TyConstr_eq_dec: forall (x y: TyConstr), { x = y } + { x <> y }.
   Proof.
     intros x y;
-      destruct x as [ n | | | ];
-      destruct y as [ m | | | ];
+      destruct x as [ n | |];
+      destruct y as [ m | |];
       solve [ left; reflexivity
             | right; intro devil; inversion devil
             | destruct (Nat.eq_dec n m) as [ eq | ineq ];
@@ -60,11 +266,38 @@ Section ClosedImplementations.
            | TyConstr_Const _ => 0
            | TyConstr_Arrow => 2
            | TyConstr_Box => 1
-           | TyConstr_BlackBox => 1
            end;
        successorVariance := fun _ _ => In |}.
 
   Definition tyConstrOrder := @eq TyConstr.
+
+  Definition tyConstrToNat (ty: TyConstr) : nat :=
+    match ty with
+    | TyConstr_Const n => cantor_sum (inl n)
+    | TyConstr_Arrow => cantor_sum (inr (cantor_sum (inl 0)))
+    | TyConstr_Box => cantor_sum (inr (cantor_sum (inr 0)))
+    end.
+  Definition natToTyConstr (n: nat) : TyConstr :=
+    match cantor_sum_inv n with
+    | inl n => TyConstr_Const n
+    | inr n =>
+      match cantor_sum_inv n with
+      | inl _ => TyConstr_Arrow
+      | inr _ => TyConstr_Box
+      end
+    end.
+  Lemma tyConstrToNat_inj: forall ty, natToTyConstr (tyConstrToNat ty) = ty.
+  Proof.
+    intro ty.
+    unfold tyConstrToNat.
+    unfold natToTyConstr.
+    destruct ty;
+      repeat rewrite cantor_sum_inj; reflexivity.
+  Qed.
+  Instance TyConstr_Countable : Countable TyConstr :=
+    {| toNat := tyConstrToNat;
+       fromNat := natToTyConstr;
+       fromTo_id := tyConstrToNat_inj |}.
   
   Inductive SigVar : Set := alpha | beta.
   Lemma SigVar_eq_dec: forall (x y: SigVar), { x = y } + { x <> y }.
@@ -74,6 +307,12 @@ Section ClosedImplementations.
       destruct y;
       solve [ left; reflexivity | right; intro devil; inversion devil ].
   Qed.
+
+  Instance SigVar_Finite : Finite SigVar :=
+    {| cardinality := 2;
+       toFin := fun x => match x with | alpha => F1 | beta => FS F1 end;
+       fromFin := fun x => match x with | F1 => alpha | Fin.FS _ => beta end;
+       fromToFin_id := fun x => match x with | alpha => eq_refl | beta  => eq_refl end |}.
 
   Inductive SigOp (from: Implementations): Set :=
   | TermOp : forall impl, List.In impl from -> SigOp from
@@ -131,7 +370,7 @@ Section ClosedImplementations.
        range :=
          fun op =>
            match op with
-           | TermOp _ impl _ => typeToSort (projT1 impl) SigVar
+           | TermOp _ impl _ => typeToSort (BoxTy (projT1 impl)) SigVar
            | ApplyOp _ => applyRange
            | MApplyOp _ => mapplyRange
            end |}.
@@ -147,10 +386,183 @@ Section ClosedImplementations.
     | _ => Const 0
     end.
 
-  Definition Carrier: VLTree TyConstr EmptySet -> Type :=
+  Lemma sortType_inj: forall ty, sortToType (typeToSort ty _) = ty.
+  Proof.
+    intro ty.
+    induction ty as [ | src IH_src tgt IH_tgt | ty IH ].
+    - reflexivity.
+    - simpl.
+      rewrite IH_src.
+      rewrite IH_tgt.
+      reflexivity.
+    - simpl; rewrite IH; reflexivity.
+  Qed.
+
+  Definition LambdaBoxCarrier: VLTree TyConstr EmptySet -> Type :=
     fun s => LambdaBox EmptyContext EmptyContext (sortToType s).    
   
 End ClosedImplementations.
+
+Module Type LambdaBoxOpsSpec.
+  Parameter EmptyContext : Fin.t 0 -> Ty.
+  Parameter Terms : @Implementations EmptyContext.
+  Parameter WellFormed: (SigVar -> @VLTree TyConstr TyConstrInfo EmptySet) -> Prop.
+End LambdaBoxOpsSpec.
+
+Module Type LambdaBoxTreeSpec(Ops: LambdaBoxOpsSpec) <: TreeSpec.
+  Definition Label := TyConstr.
+  Definition Var := SigVar.
+  Definition LOrder := tyConstrOrder.
+
+  Instance Info: LabelInfo Label := TyConstrInfo.
+  Instance LOrder_pre: PreOrder LOrder :=
+    {| PreOrder_Reflexive := eq_Reflexive; PreOrder_Transitive := eq_Transitive |}.
   
+  Definition Operation := SigOp Ops.Terms.
+  Definition WellFormed := Ops.WellFormed.
+  Instance Sigma: Signature (VLTree Label) Var Operation :=
+    MakeSignature Ops.Terms.
+
+  Definition Var_eq_dec := SigVar_eq_dec.
+  Definition Label_eq_dec := TyConstr_eq_dec.
+  Definition LOrder_dec := TyConstr_eq_dec.
+
+  Definition Vars_finite := SigVar_Finite.
+  Definition Labels_countable := TyConstr_Countable.
+  Definition GroundLabel: { l : Label | labelArity l = 0 } :=
+    exist _ (TyConstr_Const 0) (@eq_refl _ 0).
+End LambdaBoxTreeSpec.
+
+Module Type MkLambdaBoxSigSpec(Ops: LambdaBoxOpsSpec).
+  Declare Module TreeSpec: LambdaBoxTreeSpec(Ops).
+  Declare Module TreeSigSpec: TreeSignatureSpec(TreeSpec).
+  Declare Module SigSpec: TreeSortCLSignature(TreeSpec)(TreeSigSpec).
+End MkLambdaBoxSigSpec.
+
+Module Type LambdaBoxAlgebra
+       (Ops: LambdaBoxOpsSpec)
+       (MkSpec: MkLambdaBoxSigSpec(Ops))
+       (Import Alg: Algebraic(MkSpec.SigSpec)).
+  Import MkSpec.SigSpec.
+  Import MkSpec.TreeSpec.
+  Import Ops.
+
+  Lemma subst_irrelevant: forall S ty, substitute S (typeToSort ty SigVar) = typeToSort ty EmptySet.
+  Proof.
+    intros S ty.
+    induction ty as [ | src IH_src tgt IH_tgt | ty' IH ].
+    - reflexivity.
+    - simpl.
+      rewrite IH_src.
+      rewrite IH_tgt.
+      reflexivity.
+    - simpl; rewrite IH; reflexivity.
+  Qed.
+
+  Lemma subsort_eq: forall s s', subsorts s s' -> s = s'.
+  Proof.
+    intros s s'.
+    apply (fun tgt =>
+           @Fix_F_2 _ _ (fun x y => max (VLTree_size _ _ (fst x)) (VLTree_size _ _ (snd x)) <
+                                 max (VLTree_size _ _ (fst y)) (VLTree_size _ _ (snd y)))
+                    (fun x y => subsorts x y -> x = y)
+                    tgt s s' (WF_VLTree_size_max _ (s, s'))).
+    clear s s'; intros s s' IH.
+    destruct s as [ l successors | ]; [ | contradiction].
+    destruct s' as [ l' successors' | ]; [ | contradiction].
+    intro le_prf.
+    inversion le_prf
+      as [ ? ? arity_eq variance_eq ? ?  l_eq successor_prfs [ ll successors_eq ] [ ll' successors'_eq ]].
+    rewrite (vect_exist_eq _ _
+                             (existT_fg_eq (t _)
+                                           (fun l => match l with
+                                                  | TyConstr_Const _ => 0
+                                                  | TyConstr_Arrow => 2
+                                                  | TyConstr_Box => 1
+                                                  end) _ _ _ successors_eq)) in successor_prfs.
+    rewrite (vect_exist_eq _ _
+                           (existT_fg_eq (t _)
+                                         (fun l => match l with
+                                                | TyConstr_Const _ => 0
+                                                | TyConstr_Arrow => 2
+                                                | TyConstr_Box => 1
+                                                end) _ _ _ successors'_eq)) in successor_prfs.
+    revert l_eq successor_prfs IH.
+    clear ...
+    intro l_eq.
+    revert successors' arity_eq.
+    rewrite <- l_eq.
+    intros successors' arity_eq.
+    rewrite (UIP_dec (Nat.eq_dec) arity_eq eq_refl).
+    unfold eq_rect_r.
+    simpl eq_rect.
+    clear arity_eq.
+    intros successor_prfs IH.
+    apply f_equal.    
+    assert (succ_eq:
+              forall k,
+                nth successors k = nth successors' k).
+    { intro k.
+      apply IH.
+      - unfold "_ < _".
+        apply (proj1 (Nat.succ_le_mono _ _ )).
+        apply (Nat.max_le_compat).
+        + apply (proj2 (Nat.succ_le_mono _ _) (Forall_nth _ _ (VLTree_size_lt _ _ l successors) k)).
+        + apply (proj2 (Nat.succ_le_mono _ _) (Forall_nth _ _ (VLTree_size_lt _ _ l successors') k)).
+      - clear IH.
+        assert (all_in: forall k', nth (map (successorVariance l) (positions (labelArity l))) k' = In).
+        { intro k'.
+          rewrite (nth_map _ _ _ k' eq_refl).
+          reflexivity. }          
+        induction successor_prfs as [ | | | ? ? ? ? ? ? ? ? ? IH ];
+          try solve [ generalize (all_in Fin.F1); simpl; intro devil; inversion devil ].
+        + inversion k.
+        + apply (Fin.caseS' k).
+          * assumption.
+          * intro k'; apply (IH k' (fun k => all_in (Fin.FS k))). }
+    revert succ_eq.
+    clear ...
+    induction successors as [ | successor n successors IH ].
+    - intro; apply (fun r => case0 (fun xs => _ = xs) r successors'); reflexivity.
+    - apply (caseS' successors'); clear successors'; intros successor' successors'.
+      intro succ_eq.
+      generalize (succ_eq Fin.F1).
+      simpl.
+      intro successor_eq.
+      rewrite successor_eq.
+      apply f_equal.
+      apply IH.
+      exact (fun k => succ_eq (Fin.FS k)).
+  Qed.
     
-    
+  Lemma CL_Algebra: SigmaAlgebra (@LambdaBoxCarrier EmptyContext).
+  Proof.
+    unfold SigmaAlgebra.
+    intros s Fs.
+    destruct Fs as [ op subst wf_subst args subsort ].
+    unfold LambdaBoxCarrier.
+    destruct op as [ [ ty impl ] inprf | | ].
+    - generalize (subsort_eq _ _ subsort).
+      intro s_eq; clear subsort.
+      unfold range in s_eq.
+      simpl in s_eq.
+      rewrite (subst_irrelevant subst) in s_eq.
+      rewrite <- s_eq.
+      simpl.
+      rewrite sortType_inj.
+      assumption.
+    - simpl in args.
+      destruct args as [ f [ x _ ] ].
+      generalize (App _ _ _ _ f x).
+      simpl in subsort.
+      rewrite (subsort_eq _ _ subsort).
+      intro; assumption.
+    - simpl in args.
+      destruct args as [ f [ x _ ] ].
+      generalize (MApp _ _ _ _ f x).
+      simpl in subsort.
+      rewrite <- (subsort_eq _ _ subsort).
+      intro; assumption.
+  Defined.
+  
+End LambdaBoxAlgebra.
